proof.v
@@ -41,34 +41,31 @@ Section wp_span.
     iVs (cinv_cancel ⊤ graphN κ (graph_inv g markings) with "[#] [key]")
       as ">Hinv"; first done; try by iFrame.
     iClear "Hgr". unfold graph_inv.
-    iDestruct "Hinv" as (G) "Hinv";
-      iDestruct "Hinv" as (mr) "(Hi1 & Hi2 & Hi3 & Hi4 & Hi5)".
-    iDestruct "Hi4" as %Hi4. iDestruct "Hi5" as %Hi5.
+    iDestruct "Hinv" as (G) "(Hi1 & Hi2 & Hi3 & Hi4)".
+    iDestruct "Hi4" as %Hi4.
     iDestruct "H" as "[H|H]".
     - iDestruct "H" as "(_ & H)". iDestruct "H" as (l') "(H1 & H2 & Hl')".
       iDestruct "H1" as %Hl; inversion Hl; subst.
       iDestruct "H2" as (G' gmr gtr) "(Hl1 & Hl2 & Hl3 & Hl4 & Hl5)".
       iDestruct "Hl2" as %Hl2. iDestruct "Hl3" as %Hl3. iDestruct "Hl4" as %Hl4.
-      iDestruct (whole_frac with "[#]") as %Heq; [by iFrame|]; subst.
+      iDestruct (whole_frac with "[Hi1 Hl1]") as %Heq; [by iFrame|]; subst.
       iDestruct (marked_is_marked_in_auth_sepS with "[Hi2 Hl5]") as %Hmrk;
         [by iFrame|].
-      iDestruct (own_graph_valid with "#Hl1") as %Hvl.
+      iDestruct (own_graph_valid with "Hl1") as %Hvl.
       iExists (Gmon_graph G').
       assert (dom (gset positive) g = dom (gset positive) (Gmon_graph G')).
       { erewrite front_t_t_dom; eauto.
         - by rewrite Gmon_graph_dom.
-        - eapply front_mono; rewrite Gmon_graph_dom; eauto.
-          by rewrite -Hi4. }
+        - eapply front_mono; rewrite Gmon_graph_dom; eauto. }
       iVsIntro. repeat iSplitL; try by iPureIntro.
-      unfold heap_owns. rewrite of_graph_dom_eq //=.
-      by rewrite big_sepM_fmap /=.
+      rewrite /heap_owns of_graph_dom_eq //=. by rewrite big_sepM_fmap /=.
     - iDestruct "H" as "(_ & [H|H] & Hx)".
       + iDestruct "H" as %Heq. inversion Heq.
       + iDestruct "H" as (l') "(_ & Hl)".
         iDestruct (marked_is_marked_in_auth with "[Hi2 Hl]") as %Hmrk;
           [by iFrame|].
-        iDestruct (whole_frac with "[#]") as %Heq; [by iFrame|]; subst.
-        exfalso; revert Hmrk. rewrite Hi4 dom_empty. inversion 1.
+        iDestruct (whole_frac with "[Hx Hi1]") as %Heq; [by iFrame|]; subst.
+        exfalso; revert Hmrk. rewrite dom_empty. inversion 1.
   Qed.
 
 End wp_span.
